case_study/RiscvPmp/Values.v
@@ -46,71 +46,101 @@ Module RiscvPmpValueKit <: ValueKit.
   Module typekit := RiscvPmpTypeKit.
   Module Export TY := Syntax.Types.Types typekit.
 
-  Notation ty_word        := (ty_int).
-  Notation ty_regidx      := (ty_enum regidx).
-  Notation ty_rop         := (ty_enum rop).
-  Notation ty_iop         := (ty_enum iop).
-  Notation ty_uop         := (ty_enum uop).
-  Notation ty_bop         := (ty_enum bop).
-  Notation ty_retired     := (ty_enum retired).
-  Notation ty_access_type := (ty_union access_type).
+  Notation ty_word             := (ty_int).
+  Notation ty_regidx           := (ty_enum regidx).
+  Notation ty_rop              := (ty_enum rop).
+  Notation ty_iop              := (ty_enum iop).
+  Notation ty_uop              := (ty_enum uop).
+  Notation ty_bop              := (ty_enum bop).
+  Notation ty_retired          := (ty_enum retired).
+  Notation ty_access_type      := (ty_union access_type).
+  Notation ty_exception_type   := (ty_union exception_type).
+  Notation ty_memory_op_result := (ty_union memory_op_result).
 
   (** Unions **)
   Definition 𝑼𝑲_Ty (U : 𝑼) : 𝑼𝑲 U -> Ty :=
     match U with
-    | ast => fun K =>
-               match K with
-               | KRTYPE      => ty_tuple [ty_regidx, ty_regidx, ty_regidx, ty_rop]
-               | KITYPE      => ty_tuple [ty_int, ty_regidx, ty_regidx, ty_iop]
-               | KUTYPE      => ty_tuple [ty_int, ty_regidx, ty_uop]
-               | KBTYPE      => ty_tuple [ty_int, ty_regidx, ty_regidx, ty_bop]
-               | KRISCV_JAL  => ty_tuple [ty_int, ty_regidx]
-               | KRISCV_JALR => ty_tuple [ty_int, ty_regidx, ty_regidx]
-               | KLOAD       => ty_tuple [ty_int, ty_regidx, ty_regidx]
-               end
-    | access_type => fun K => ty_unit
+    | ast              => fun K =>
+                            match K with
+                            | KRTYPE      => ty_tuple [ty_regidx, ty_regidx, ty_regidx, ty_rop]
+                            | KITYPE      => ty_tuple [ty_int, ty_regidx, ty_regidx, ty_iop]
+                            | KUTYPE      => ty_tuple [ty_int, ty_regidx, ty_uop]
+                            | KBTYPE      => ty_tuple [ty_int, ty_regidx, ty_regidx, ty_bop]
+                            | KRISCV_JAL  => ty_tuple [ty_int, ty_regidx]
+                            | KRISCV_JALR => ty_tuple [ty_int, ty_regidx, ty_regidx]
+                            | KLOAD       => ty_tuple [ty_int, ty_regidx, ty_regidx]
+                            end
+    | access_type      => fun _ => ty_unit
+    | exception_type   => fun _ => ty_unit
+    | memory_op_result => fun K =>
+                            match K with
+                            | KMemValue     => ty_word
+                            | KMemException => ty_exception_type
+                            end
     end.
 
   Definition 𝑼_unfold (U : 𝑼) : 𝑼𝑻 U -> { K : 𝑼𝑲 U & Lit (𝑼𝑲_Ty U K) } :=
     match U as u return (𝑼𝑻 u -> {K : 𝑼𝑲 u & Lit (𝑼𝑲_Ty u K)}) with
-    | ast => fun Kv =>
-               match Kv with
-               | RTYPE rs2 rs1 rd op   => existT KRTYPE (tt , rs2 , rs1 , rd , op)
-               | ITYPE imm rs1 rd op   => existT KITYPE (tt , imm , rs1 , rd , op)
-               | UTYPE imm rd op       => existT KUTYPE (tt , imm , rd , op)
-               | BTYPE imm rs2 rs1 op  => existT KBTYPE (tt , imm , rs2 , rs1 , op)
-               | RISCV_JAL imm rd      => existT KRISCV_JAL (tt , imm , rd)
-               | RISCV_JALR imm rs1 rd => existT KRISCV_JALR (tt , imm , rs1 , rd)
-               | LOAD imm rs1 rd       => existT KLOAD (tt , imm , rs1 , rd)
-               end
-    | access_type => fun Kv =>
-                       match Kv with
-                       | Read      => existT KRead tt
-                       | Write     => existT KWrite tt
-                       | ReadWrite => existT KReadWrite tt
-                       | Execute   => existT KExecute tt
-                       end
+    | ast              => fun Kv =>
+                            match Kv with
+                            | RTYPE rs2 rs1 rd op   => existT KRTYPE (tt , rs2 , rs1 , rd , op)
+                            | ITYPE imm rs1 rd op   => existT KITYPE (tt , imm , rs1 , rd , op)
+                            | UTYPE imm rd op       => existT KUTYPE (tt , imm , rd , op)
+                            | BTYPE imm rs2 rs1 op  => existT KBTYPE (tt , imm , rs2 , rs1 , op)
+                            | RISCV_JAL imm rd      => existT KRISCV_JAL (tt , imm , rd)
+                            | RISCV_JALR imm rs1 rd => existT KRISCV_JALR (tt , imm , rs1 , rd)
+                            | LOAD imm rs1 rd       => existT KLOAD (tt , imm , rs1 , rd)
+                            end
+    | access_type      => fun Kv =>
+                            match Kv with
+                            | Read      => existT KRead tt
+                            | Write     => existT KWrite tt
+                            | ReadWrite => existT KReadWrite tt
+                            | Execute   => existT KExecute tt
+                            end
+    | exception_type   => fun Kv =>
+                            match Kv with
+                            | E_FETCH_ACCESS_FAULT => existT KE_FETCH_ACCESS_FAULT tt
+                            | E_LOAD_ACCESS_FAULT  => existT KE_LOAD_ACCESS_FAULT tt
+                            | E_SAMO_ACCESS_FAULT  => existT KE_SAMO_ACCESS_FAULT tt
+                            end
+    | memory_op_result => fun Kv =>
+                            match Kv with
+                            | MemValue v => existT KMemValue v
+                            | MemException e => existT KMemException e
+                            end
     end.
 
   Definition 𝑼_fold (U : 𝑼) : { K : 𝑼𝑲 U & Lit (𝑼𝑲_Ty U K) } -> 𝑼𝑻 U :=
     match U with
-    | ast => fun Kv =>
-               match Kv with
-               | existT KRTYPE (tt , rs2 , rs1 , rd , op)  => RTYPE rs2 rs1 rd op
-               | existT KITYPE (tt , imm , rs1 , rd , op)  => ITYPE imm rs1 rd op
-               | existT KUTYPE (tt , imm , rd , op)        => UTYPE imm rd op
-               | existT KBTYPE (tt , imm , rs2 , rs1 , op) => BTYPE imm rs2 rs1 op
-               | existT KRISCV_JAL (tt , imm , rd)         => RISCV_JAL imm rd
-               | existT KRISCV_JALR (tt , imm , rs1 , rd)  => RISCV_JALR imm rs1 rd
-               | existT KLOAD (tt , imm , rs1 , rd)        => LOAD imm rs1 rd
-               end
-    | access_type => fun Kv =>
-                       match Kv with
-                       | existT KRead tt      => Read
-                       | existT KWrite tt     => Write
-                       | existT KReadWrite tt => ReadWrite
-                       | existT KExecute tt   => Execute
-                       end
+    | ast              => fun Kv =>
+                            match Kv with
+                            | existT KRTYPE (tt , rs2 , rs1 , rd , op)  => RTYPE rs2 rs1 rd op
+                            | existT KITYPE (tt , imm , rs1 , rd , op)  => ITYPE imm rs1 rd op
+                            | existT KUTYPE (tt , imm , rd , op)        => UTYPE imm rd op
+                            | existT KBTYPE (tt , imm , rs2 , rs1 , op) => BTYPE imm rs2 rs1 op
+                            | existT KRISCV_JAL (tt , imm , rd)         => RISCV_JAL imm rd
+                            | existT KRISCV_JALR (tt , imm , rs1 , rd)  => RISCV_JALR imm rs1 rd
+                            | existT KLOAD (tt , imm , rs1 , rd)        => LOAD imm rs1 rd
+                            end
+    | access_type      => fun Kv =>
+                            match Kv with
+                            | existT KRead tt      => Read
+                            | existT KWrite tt     => Write
+                            | existT KReadWrite tt => ReadWrite
+                            | existT KExecute tt   => Execute
+                            end
+    | exception_type   => fun Kv =>
+                            match Kv with
+                            | existT KE_FETCH_ACCESS_FAULT tt => E_FETCH_ACCESS_FAULT
+                            | existT KE_LOAD_ACCESS_FAULT tt  => E_LOAD_ACCESS_FAULT
+                            | existT KE_SAMO_ACCESS_FAULT tt  => E_SAMO_ACCESS_FAULT
+                            end
+    | memory_op_result => fun Kv =>
+                            match Kv with
+                            | existT KMemValue v => MemValue v
+                            | existT KMemException e => MemException e
+                            end
     end.
 
   Lemma 𝑼_fold_unfold : forall (U : 𝑼) (Kv: 𝑼𝑻 U),
